Updated Juliano's hardware compilation to work with wordsTheory.  There are now some nasty parser warnings with "===>", "<>" and possibly others.
The dev/booth example was/is broken (I haven't attempted to repair it).

Have updated dev/AES/word8 and Crypto/AES.  Perhaps dev/AES should be removed?

The hardware compilation for Crypto/TEA and Crypto/RC6 are now broken.
Updating the Crypto examples should be straightforward.  Once done I can
delete src/n_bit.

examples/dev/AES/word8/word8CasesLib.sig
@@ -1,9 +1,0 @@
-signature word8CasesLib = sig
-
-include Abbrev
-
- val word8Define : term quotation -> thm
- val word8Cases_on : term quotation -> tactic
- val word8GenCases : term quotation -> (term -> thm) -> (thm * thm)
-
-end
