examples/dev/compile.sml
@@ -18,8 +18,8 @@ open arithmeticTheory pairLib pairTheory PairRules pairSyntax
      combinTheory listTheory unwindLib composeTheory compileTheory;
 
 loadPath := "Fact32" :: !loadPath;
-map load ["word32Theory","word32Lib","compile"];
-open word32Theory word32Lib compile ;
+map load ["wordsLib","compile"];
+open wordsTheory wordsLib compile ;
 
 quietdec := false;
 *)
@@ -1925,7 +1925,7 @@ fun FUN_EXISTS_PROD_CONV tm =
        val ty2list = strip_prod ty2
        val vartys = map (curry op--> ty1) ty2list
        val init_vars = map mk_var 
-                        (zip (map (concat "f_" o Int.toString) 
+                        (zip (map (strcat "f_" o Int.toString) 
                                   (upto 1 (length vartys)))
                              vartys)
        val vars = variants (free_vars tm) init_vars
