examples/Crypto/AES/aesScript.sml
@@ -64,37 +64,37 @@ val DUMMY_KEYS_def =
 (* Orchestrate the round computations.                                       *)
 (*---------------------------------------------------------------------------*)
 
-val RoundTuple_def = 
- Define
-   `RoundTuple (n:num,keys:keysched,state:state) = 
-     if n=0 
+val (RoundTuple_def, RoundTuple_ind) = Defn.tprove
+ (Hol_defn
+   "RoundTuple"
+   `RoundTuple (n, keys:keysched, state:state) =
+     if n=0
       then (0,ROTKEYS keys,
-            AddRoundKey (FST keys) 
-               (ShiftRows (SubBytes state)))
-      else RoundTuple (n-1,ROTKEYS keys,
-                  AddRoundKey (FST keys) 
-                    (MixColumns 
-                      (ShiftRows 
-                         (SubBytes state))))`;
+            AddRoundKey (FST keys)
+              (ShiftRows (SubBytes state)))
+      else RoundTuple (n-1, ROTKEYS keys,
+            (AddRoundKey (FST keys)
+              (MixColumns (ShiftRows (SubBytes state)))))`,
+  WF_REL_TAC `measure FST` THEN REPEAT PairRules.PGEN_TAC THEN DECIDE_TAC);
 
-
-val InvRoundTuple_def = 
- Define
-   `InvRoundTuple (n:num,keys:keysched,state:state) =
-      if n=0 
+val (InvRoundTuple_def,InvRoundTuple_ind) = Defn.tprove
+ (Hol_defn
+   "InvRoundTuple"
+   `InvRoundTuple (n, keys:keysched, state:state) =
+      if n=0
        then (0,ROTKEYS keys,
-             AddRoundKey (FST keys) 
-                 (InvSubBytes (InvShiftRows state)))
+             AddRoundKey (FST keys)
+               (InvSubBytes (InvShiftRows state)))
        else InvRoundTuple (n-1,ROTKEYS keys,
-                     InvMixColumns 
-                       (AddRoundKey (FST keys) 
-                         (InvSubBytes 
-                           (InvShiftRows state))))`;
+             (InvMixColumns
+               (AddRoundKey (FST keys)
+                 (InvSubBytes (InvShiftRows state)))))`,
+  WF_REL_TAC `measure FST` THEN REPEAT PairRules.PGEN_TAC THEN DECIDE_TAC);
 
-
-val Round_def = Define `Round n k s = SND(SND(RoundTuple(n,k,s)))`;
-val InvRound_def = Define `InvRound n k s = SND(SND(InvRoundTuple(n,k,s)))`;
-
+val _ = save_thm ("RoundTuple_def", RoundTuple_def);
+val _ = save_thm ("RoundTuple_ind", RoundTuple_ind);
+val _ = save_thm ("InvRoundTuple_def", InvRoundTuple_def);
+val _ = save_thm ("InvRoundTuple_ind", InvRoundTuple_ind);
 
 val Round_def = Define `Round n k s = SND(SND(RoundTuple(n,k,s)))`;
 val InvRound_def = Define `InvRound n k s = SND(SND(InvRoundTuple(n,k,s)))`;
@@ -103,16 +103,16 @@ val InvRound_def = Define `InvRound n k s = SND(SND(InvRoundTuple(n,k,s)))`;
 (* Encrypt and Decrypt                                                       *)
 (*---------------------------------------------------------------------------*)
 
-val AES_FWD_def = 
- Define 
-  `AES_FWD keys = 
-    from_state o Round 9 (ROTKEYS keys) 
+val AES_FWD_def =
+ Define
+  `AES_FWD keys =
+    from_state o Round 9 (ROTKEYS keys)
                o AddRoundKey (FST keys) o to_state`;
-     
-val AES_BWD_def = 
- Define 
-  `AES_BWD keys = 
-    from_state o InvRound 9 (ROTKEYS keys) 
+
+val AES_BWD_def =
+ Define
+  `AES_BWD keys =
+    from_state o InvRound 9 (ROTKEYS keys)
                o AddRoundKey (FST keys) o to_state`;
      
 (*---------------------------------------------------------------------------*)
@@ -125,15 +125,14 @@ val [genMixColumns] = decls "genMixColumns";
 
 val AES_LEMMA = Q.store_thm
 ("AES_LEMMA",
- `!(plaintext:state) (keys:keysched). 
+ `!(plaintext:state) (keys:keysched).
      AES_BWD (REVKEYS keys) (AES_FWD keys plaintext) = plaintext`,
- SIMP_TAC std_ss [FORALL_BLOCK] THEN 
+ SIMP_TAC std_ss [FORALL_BLOCK] THEN
  SIMP_TAC std_ss [FORALL_KEYSCHED]
    THEN RESTR_EVAL_TAC [MultCol,InvMultCol,genMixColumns]
    THEN RW_TAC std_ss [ShiftRows_Inversion,SubBytes_Inversion,
                        XOR_BLOCK_IDEM,MixColumns_Inversion,
                        from_state_Inversion,from_state_def]);
-
 
 (*---------------------------------------------------------------------------
      Generate the key schedule from key. We work using 4-tuples of
@@ -146,7 +145,7 @@ val _ = set_fixity "XOR8x4"  (Infixr 350);
 
 val XOR8x4_def = 
  Define 
-   `(a,b,c,d) XOR8x4 (a1,b1,c1,d1) = (a # a1, b # b1, c # c1, d # d1)`;
+   `(a,b,c,d) XOR8x4 (a1,b1,c1,d1) = (a ?? a1, b ?? b1, c ?? c1, d ?? d1)`;
 
 val SubWord_def = Define 
    `SubWord(b0,b1,b2,b3) = (Sbox b0, Sbox b1, Sbox b2, Sbox b3)`;
@@ -195,13 +194,20 @@ val mk_keysched_def = Define
 (* Sanity check                                                              *)
 (*---------------------------------------------------------------------------*)
 val _ = Globals.priming := SOME"";
+
+(*
+val PolyExp = Q.prove
+(`(PolyExp x 0 = 1w) /\
+  (PolyExp x (SUC n) = x ** PolyExp x n)`,
+*)
+
 (*
 val keysched_length = Count.apply Q.prove
 (`!key. LENGTH (mk_keysched key) = 11`,
  SIMP_TAC std_ss [FORALL_BLOCK,mk_keysched_def]
   THEN REPEAT GEN_TAC 
   THEN NTAC 42
-     (fn x => (RW_TAC list_ss [Once expand_def] 
+     (fn x => (RW_TAC list_ss [Once expand_def,LET_THM] 
        THEN FULL_SIMP_TAC list_ss [markerTheory.Abbrev_def]
        THEN RW_TAC list_ss [XOR8x4_def, SubWord_def, RotWord_def, Rcon_def,
                             tablesTheory.Sbox_def,MultTheory.PolyExp_def]) x)
@@ -221,10 +227,9 @@ RW_TAC list_ss [unpack_def]
 (*---------------------------------------------------------------------------*)
 
 val AES_def = Define
- `AES key = 
-   let keys = LIST_TO_KEYS (mk_keysched key) DUMMY_KEYS 
+ `AES key =
+   let keys = LIST_TO_KEYS (mk_keysched key) DUMMY_KEYS
    in (AES_FWD keys, AES_BWD (REVKEYS keys))`;
-
 
 (*---------------------------------------------------------------------------*)
 (* Basic theorem about encryption/decryption                                 *)
