examples/dev/AES/word8/MultScript.sml
@@ -4,27 +4,16 @@
 (*---------------------------------------------------------------------------*)
 
 (* For interactive work
-  app load ["word8Theory", "metisLib", "word8CasesLib"];
+  load "wordsLib";
   quietdec := true;
-  open word8Theory bitsTheory
-     word8Lib arithmeticTheory metisLib word8CasesLib;
+  open wordsTheory bitTheory wordsLib arithmeticTheory;
   quietdec := false;
 *)
 
 open HolKernel Parse boolLib bossLib 
-     word8Theory bitsTheory
-     word8Lib arithmeticTheory metisLib word8CasesLib;
+     wordsTheory bitTheory wordsLib arithmeticTheory;
 
 val _ = new_theory "Mult";
-
-fun n2w_TAC v = STRIP_ASSUME_TAC (Q.SPEC v word_nchotomy) THEN
-                ASM_REWRITE_TAC []
-
-val EQ_BIT_THM = Q.prove (
-`!a b. (a = b) = (!n. n < 8 ==> (WORD_BIT n a = WORD_BIT n b))`,
-REPEAT STRIP_TAC THEN n2w_TAC `a` THEN n2w_TAC `b` THEN
-RW_TAC arith_ss [BIT_EVAL, n2w_11, w2n_EVAL, MOD_WL_THM, GSYM BIT_BITS_THM,
-                 HB_def, LE_LT1, BIT_OF_BITS_THM])
 
 (*---------------------------------------------------------------------------
     Multiply a byte (representing a polynomial) by x. 
@@ -33,31 +22,16 @@ RW_TAC arith_ss [BIT_EVAL, n2w_11, w2n_EVAL, MOD_WL_THM, GSYM BIT_BITS_THM,
 
 val xtime_def = Define
   `xtime (w : word8) =
-     w << 1 # (if MSB w then
-                 0x1Bw
-               else
-                 0w)`;
+     w << 1 ?? (if word_msb w then 0x1Bw else 0w)`;
 
 val MSB_lem = Q.prove (
-`!a b. MSB (a # b) = ~(MSB a = MSB b)`,
-REPEAT STRIP_TAC THEN n2w_TAC `a` THEN n2w_TAC `b` THEN 
-RW_TAC arith_ss [EOR_EVAL, EOR_def, MSB_EVAL, MSBn_def, HB_def, WL_def,
-                 BITWISE_THM]);
+  `!a b. word_msb (a ?? b) = ~(word_msb a = word_msb b)`,
+  SRW_TAC [WORD_BIT_EQ_ss] []);
 
 val xtime_distrib = Q.store_thm
 ("xtime_distrib",
- `!a b. xtime (a # b) = xtime a # xtime b`,
- RW_TAC std_ss [EQ_BIT_THM, xtime_def, MSB_lem, WORD_EOR_ID] THEN
- FULL_SIMP_TAC std_ss [] THEN RW_TAC std_ss [] THEN
- n2w_TAC `a` THEN n2w_TAC `b` THEN
- RW_TAC arith_ss [BIT_EVAL, EOR_EVAL, LSL_EVAL, HB_def, MUL_EVAL, w2n_EVAL,
-                  MOD_WL_THM, MIN_DEF, BIT_OF_BITS_THM, EOR_def, WL_def,
-                  BITWISE_THM] THEN
- PURE_ONCE_REWRITE_TAC [Q.prove (`!a. a * 2 = a * 2 ** 1`, RW_TAC arith_ss [])]
- THEN
- Cases_on `n<1` THEN
- FULL_SIMP_TAC arith_ss [BIT_SHIFT_THM3, NOT_LESS, BIT_SHIFT_THM2, BITWISE_THM] THEN
- METIS_TAC []);
+ `!a b. xtime (a ?? b) = xtime a ?? xtime b`,
+  SRW_TAC [] [xtime_def, MSB_lem] THEN FULL_SIMP_TAC std_ss []);
 
 (*---------------------------------------------------------------------------*)
 (* Multiplication by a constant                                              *)
@@ -69,15 +43,11 @@ val (ConstMult_def,ConstMult_ind) =
  Defn.tprove
   (Hol_defn "ConstMult"
      `b1 ** b2 =
-        if b1 = 0w then 0w else 
-        if LSB b1
-           then b2 # ((b1 >>> 1) ** xtime b2)
-           else      ((b1 >>> 1) ** xtime b2)`,
-   WF_REL_TAC `measure (w2n o FST)` THEN 
-   (* It would be nice to use LSR1_LESS instead of brute force, but
-      I didn't finish proving it.  *)
-   STRIP_TAC THEN word8Cases_on `b1` THEN 
-   RW_TAC std_ss [] THEN REPEAT (POP_ASSUM MP_TAC) THEN WORD_TAC)
+        if b1 = 0w:word8 then 0w else 
+        if word_lsb b1
+           then b2 ?? ((b1 >>> 1) ** xtime b2)
+           else       ((b1 >>> 1) ** xtime b2)`,
+   WF_REL_TAC `measure (w2n o FST)`);
 
 val _ = save_thm("ConstMult_def",ConstMult_def);
 val _ = save_thm("ConstMult_ind",ConstMult_ind);
@@ -85,12 +55,11 @@ val _ = computeLib.add_persistent_funs [("ConstMult_def",ConstMult_def)];
 
 val ConstMultDistrib = Q.store_thm
 ("ConstMultDistrib",
- `!x y z. x ** (y # z) = (x ** y) # (x ** z)`,
+ `!x y z. x ** (y ?? z) = (x ** y) ?? (x ** z)`,
  recInduct ConstMult_ind
    THEN REPEAT STRIP_TAC
    THEN ONCE_REWRITE_TAC [ConstMult_def]
-   THEN RW_TAC std_ss [xtime_distrib, AC WORD_EOR_ASSOC WORD_EOR_COMM]
-   THEN WORD_TAC);
+   THEN SRW_TAC [] [xtime_distrib]);
 
 (*---------------------------------------------------------------------------*)
 (* Iterative version                                                         *)
@@ -99,16 +68,13 @@ val ConstMultDistrib = Q.store_thm
 val defn = Hol_defn 
   "IterConstMult"
   `IterConstMult (b1,b2,acc) =
-     if b1 = 0w then (b1,b2,acc)
+     if b1 = 0w:word8 then (b1,b2,acc)
      else IterConstMult (b1 >>> 1, xtime b2,
-                         if LSB b1 then (b2 # acc) else acc)`;
+                         if word_lsb b1 then (b2 ?? acc) else acc)`;
 
 val (IterConstMult_def,IterConstMult_ind) = 
  Defn.tprove
-  (defn,
-   WF_REL_TAC `measure (w2n o FST)` THEN STRIP_TAC THEN
-   word8Cases_on `b1` THEN 
-   RW_TAC std_ss [] THEN REPEAT (POP_ASSUM MP_TAC) THEN WORD_TAC);
+  (defn, WF_REL_TAC `measure (w2n o FST)`);
 
 val _ = save_thm("IterConstMult_def",IterConstMult_def);
 val _ = save_thm("IterConstMult_ind",IterConstMult_ind);
@@ -120,12 +86,10 @@ val _ = computeLib.add_persistent_funs [("IterConstMult_def",IterConstMult_def)]
 
 val ConstMultEq = Q.store_thm
 ("ConstMultEq",
- `!b1 b2 acc. (b1 ** b2) # acc = SND(SND(IterConstMult (b1,b2,acc)))`,
+ `!b1 b2 acc. (b1 ** b2) ?? acc = SND(SND(IterConstMult (b1,b2,acc)))`,
  recInduct IterConstMult_ind THEN RW_TAC std_ss []
    THEN ONCE_REWRITE_TAC [ConstMult_def,IterConstMult_def]
-   THEN RW_TAC std_ss [AC WORD_EOR_ASSOC WORD_EOR_COMM]
-   THEN FULL_SIMP_TAC std_ss [AC WORD_EOR_ASSOC WORD_EOR_COMM, WORD_EOR_ID]);
-
+   THEN FULL_SIMP_TAC (srw_ss()) [] THEN SRW_TAC [] []);
 
 (*---------------------------------------------------------------------------*)
 (* Tabled versions                                                           *)
@@ -137,32 +101,10 @@ fun UNROLL_RULE 0 def = def
      (GEN_REWRITE_RULE (RHS_CONV o DEPTH_CONV) empty_rewrites [def]
                        (UNROLL_RULE (n - 1) def))
 val instantiate =
- SIMP_RULE arith_ss [WORD_EOR_ID, GSYM xtime_distrib] o 
- WORD_RULE o
+ SIMP_RULE (srw_ss()) [WORD_XOR_CLAUSES, GSYM xtime_distrib] o 
  ONCE_REWRITE_CONV [UNROLL_RULE 4 ConstMult_def]
 
 val IterMult2 = UNROLL_RULE 1 IterConstMult_def
-
-val mult_thm =
-LIST_CONJ (map instantiate [``0x2w ** x``, ``0x3w ** x``, ``0x9w ** x``,
-                            ``0xBw ** x``, ``0xDw ** x``, ``0xEw ** x``])
-
-val eval_mult =
-WORD_RULE o PURE_REWRITE_CONV [mult_thm, xtime_def]
-
-fun build_table arg1 = word8GenCases `$** ^arg1` eval_mult
-
-(*---------------------------------------------------------------------------*)
-(* Construct specialized multiplication tables.                              *)
-(*---------------------------------------------------------------------------*)
-
-val (mult_tables, mult_ifs) =
-let val (ifs, tables) =
-        unzip (map (Count.apply build_table)
-               [``0x2w``, ``0x3w``, ``0x9w``, ``0xBw``, ``0xDw``, ``0xEw``])
-in
-(LIST_CONJ tables, LIST_CONJ ifs)
-end
 
 (*---------------------------------------------------------------------------*)
 (* mult_unroll                                                               *)
@@ -174,7 +116,24 @@ end
 (*       (14w ** x = xtime (x # xtime (x # xtime x)))                        *)
 (*---------------------------------------------------------------------------*)
 
-val _ = save_thm ("mult_unroll", mult_thm)
+val mult_unroll = save_thm("mult_unroll",
+  LIST_CONJ (map instantiate
+    [``0x2w ** x``, ``0x3w ** x``, ``0x9w ** x``,
+     ``0xBw ** x``, ``0xDw ** x``, ``0xEw ** x``]));
+
+val eval_mult = WORD_EVAL_RULE o PURE_REWRITE_CONV [mult_unroll, xtime_def]
+
+fun mk_word8 i = wordsSyntax.mk_n2w(numSyntax.term_of_int i, ``:8``);
+
+(*---------------------------------------------------------------------------*)
+(* Construct specialized multiplication tables.                              *)
+(*---------------------------------------------------------------------------*)
+
+val mult_tables =
+  LIST_CONJ (List.concat (map (fn x => List.tabulate(256,
+       fn i => let val y = mk_word8 i in eval_mult ``^x ** ^y`` end))
+  [``0x2w:word8``, ``0x3w:word8``, ``0x9w:word8``,
+   ``0xBw:word8``, ``0xDw:word8``, ``0xEw:word8``]));
 
 (*---------------------------------------------------------------------------*)
 (* Multiplication by constant implemented by one-step rewrites.              *)
@@ -187,7 +146,9 @@ val _ = save_thm ("mult_tables", mult_tables)
 (* tree. Lookup is done bit-by-bit.                                          *)
 (*---------------------------------------------------------------------------*)
 
+(*
 val _ = save_thm ("mult_ifs", mult_ifs)
+*)
  
 (*---------------------------------------------------------------------------*)
 (* Exponentiation                                                            *)
